ref_impl/src/verifier/fstar_files/util.fst
@@ -5,3 +5,5 @@ let max x y = if (x > y) then x else y
 
 val min : nat -> nat -> nat
 let min x y = if (x > y) then y else x
+
+assume val cast (t1 : Type) (t2 : Type) (a : t1) : t2
