ref_impl/src/verifier/provingEquivalence.fst
@@ -1,0 +1,17 @@
+module ProvingEquivalence
+
+
+val isZero : n:nat -> Tot bool
+let rec isZero x = if (x = 0) then true else false
+
+val f : n:nat{isZero n} -> n:nat{n=1}
+let f x = x + 1
+
+val isZero2 : n:nat -> Tot bool
+let rec isZero2 x = if (x = 0) then true else if (x = 1) then false else isZero2 (x - 1)
+
+val lemmaIsZeroEquiv : n:nat -> Lemma (ensures (isZero n) = (isZero2 n))
+let rec lemmaIsZeroEquiv n = if (n = 0) then () else lemmaIsZeroEquiv (n - 1)
+
+val f2 : n:nat{isZero n} -> n:nat{n=1}
+let f2 x = lemmaIsZeroEquiv x; x + 1
