ref_impl/src/verifier/fstar_files/NSMain__main_main_didntwork.fst~
@@ -6,17 +6,18 @@ open Util
 
 (* Type names *)
 let bTypedStringType_BAnyType = (BTypedStringType BAnyType)
+let bTypedStringType_BNoneType = (BTypedStringType BNoneType)
 let bTupleType_2BIntType_BIntTypefalse = BTupleType false 2 (SCons BIntType 1 (SCons BIntType 0 SNil))
 let bTupleType_2BIntType_bTupleType_2BIntType_BIntTypefalsefalse = BTupleType false 2 (SCons BIntType 1 (SCons bTupleType_2BIntType_BIntTypefalse 0 SNil))
 let bTupleType_3bTupleType_2BIntType_BIntTypefalse_bTupleType_2BIntType_BIntTypefalse_BIntTypefalse = BTupleType false 3 (SCons bTupleType_2BIntType_BIntTypefalse 2 (SCons bTupleType_2BIntType_BIntTypefalse 1 (SCons BIntType 0 SNil)))
 let bTupleType_16BIntType_BIntType_BIntType_BIntType_BIntType_BIntType_BIntType_BIntType_BIntType_BIntType_BIntType_BIntType_bTupleType_2BIntType_BIntTypefalse_bTypedStringType_BAnyType_BBoolType_BBoolTypefalse = BTupleType false 16 (SCons BIntType 15 (SCons BIntType 14 (SCons BIntType 13 (SCons BIntType 12 (SCons BIntType 11 (SCons BIntType 10 (SCons BIntType 9 (SCons BIntType 8 (SCons BIntType 7 (SCons BIntType 6 (SCons BIntType 5 (SCons BIntType 4 (SCons bTupleType_2BIntType_BIntTypefalse 3 (SCons bTypedStringType_BAnyType 2 (SCons BBoolType 1 (SCons BBoolType 0 SNil))))))))))))))))
-let bUnionType_BBoolType_BIntType_BNoneType_bTypedStringType_BAnyType = (BUnionType BBoolType (BUnionType BIntType (BUnionType BNoneType bTypedStringType_BAnyType)))
+let bUnionType_BBoolType_BIntType_BNoneType_bTypedStringType_BNoneType = (BUnionType BBoolType (BUnionType BIntType (BUnionType BNoneType bTypedStringType_BNoneType)))
 let bUnionType_BIntType_BNoneType = (BUnionType BIntType BNoneType)
 let bTupleType_3BIntType_BBoolType_BIntTypefalse = BTupleType false 3 (SCons BIntType 2 (SCons BBoolType 1 (SCons BIntType 0 SNil)))
 let bTupleType_4BIntType_BBoolType_BIntType_BBoolTypetrue = BTupleType true 4 (SCons BIntType 3 (SCons BBoolType 2 (SCons BIntType 1 (SCons BBoolType 0 SNil))))
 let bUnionType_bTupleType_3BIntType_BBoolType_BIntTypefalse_bTupleType_4BIntType_BBoolType_BIntType_BBoolTypetrue = (BUnionType bTupleType_3BIntType_BBoolType_BIntTypefalse bTupleType_4BIntType_BBoolType_BIntType_BBoolTypetrue)
 let bTupleType_1bTypedStringType_BAnyTypefalse = BTupleType false 1 (SCons bTypedStringType_BAnyType 0 SNil)
-let bTupleType_1bTypedStringType_BAnyTypetrue = BTupleType true 1 (SCons bTypedStringType_BAnyType 0 SNil)
+let bTupleType_1bTypedStringType_BNoneTypetrue = BTupleType true 1 (SCons bTypedStringType_BNoneType 0 SNil)
 let bUnionType_BBoolType_BNoneType = (BUnionType BBoolType BNoneType)
 let bUnionType_BBoolType_BIntType_BNoneType = (BUnionType BBoolType (BUnionType BIntType BNoneType))
 let bUnionType_BBoolType_BNoneType_BIntType = (BUnionType BBoolType (BUnionType BNoneType BIntType))
@@ -27,20 +28,6 @@ let bTupleType_2BIntType_bUnionType_BBoolType_BNoneTypefalse = BTupleType false 
 (* Concept Declarations *)
 
 (* Entity Declarations *)
-type nSMain__Musician = 
-| BnSMain__Musician : artist : nSMain__Artist -> 
-instrument : bosqueTerm{bTypedStringType_BAnyType = (getType instrument)} -> 
-nSMain__Musician
-type nSMain__Artist = 
-| BnSMain__Artist : id : bosqueTerm{BIntType = (getType id)} -> 
-isGood : bosqueTerm{BBoolType = (getType isGood)} -> 
-lastName : bosqueTerm{bTypedStringType_BAnyType = (getType lastName)} -> 
-name : bosqueTerm{bTypedStringType_BAnyType = (getType name)} -> 
-player : nSMain__PlayerMark -> 
-nSMain__Artist
-type nSMain__PlayerMark = 
-| BnSMain__PlayerMark : mark : bosqueTerm{bTypedStringType_BAnyType = (getType mark)} -> 
-nSMain__PlayerMark
 
 (* Constant Declarations *)
 
@@ -63,7 +50,7 @@ let nSMain__max3 x =
         let _return_ = __ir_ret___2 in 
          _return_
 
-val nSMain__identityUnion : (x:bosqueTerm{subtypeOf bUnionType_BBoolType_BIntType_BNoneType_bTypedStringType_BAnyType (getType x)}) -> Tot (x:bosqueTerm{subtypeOf bUnionType_BBoolType_BIntType_BNoneType_bTypedStringType_BAnyType (getType x)})
+val nSMain__identityUnion : (x:bosqueTerm{subtypeOf bUnionType_BBoolType_BIntType_BNoneType_bTypedStringType_BNoneType (getType x)}) -> Tot (x:bosqueTerm{subtypeOf bUnionType_BBoolType_BIntType_BNoneType_bTypedStringType_BNoneType (getType x)})
 let nSMain__identityUnion x = 
  let __ir_ret__ = x in 
   let _return_ = __ir_ret__ in 
@@ -96,7 +83,7 @@ let nSMain__identityTupleOptional x =
   let _return_ = __ir_ret__ in 
    _return_
 
-val nSMain__identityOpenTuple : (x:bosqueTerm{subtypeOf bTupleType_1bTypedStringType_BAnyTypetrue (getType x)}) -> Tot (x:bosqueTerm{subtypeOf bTupleType_1bTypedStringType_BAnyTypetrue (getType x)})
+val nSMain__identityOpenTuple : (x:bosqueTerm{subtypeOf bTupleType_1bTypedStringType_BNoneTypetrue (getType x)}) -> Tot (x:bosqueTerm{subtypeOf bTupleType_1bTypedStringType_BNoneTypetrue (getType x)})
 let nSMain__identityOpenTuple x = 
  let __ir_ret__ = x in 
   let _return_ = __ir_ret__ in 
@@ -121,6 +108,20 @@ let nSMain__identityTupleNoneable x =
  let __ir_ret__ = x in 
   let _return_ = __ir_ret__ in 
    _return_
+
+type playerMark =
+| BnSMain__PlayerMark : x : bosqueTerm{subtypeOf (BTypedStringType BAnyType) (getType x)} -> playerMark 
+
+type artist =
+| BnSMain__Artist : x1 : bosqueTerm{subtypeOf (BIntType) (getType x1)}
+-> x2 : bosqueTerm{subtypeOf (BBoolType) (getType x2)}
+-> x3 : bosqueTerm{subtypeOf (BTypedStringType BAnyType) (getType x3)}
+-> x4 : bosqueTerm{subtypeOf (BTypedStringType BAnyType) (getType x4)}
+-> x5 : playerMark
+-> artist 
+
+type musician = 
+| BnSMain__Musician : x1 : artist -> x2 : bosqueTerm{subtypeOf (BTypedStringType BAnyType) (getType x2)} -> musician
 
 val nSMain__main : (x:bosqueTerm{subtypeOf BIntType (getType x)})
 let nSMain__main  = 
